doc/simple/coq/CtxExtension.v
@@ -1240,15 +1240,7 @@ Proof.
   rewrite HH in H0. apply AWf_push_inv in H0. auto_star.
 Qed.
 
-Lemma extension_weakening_awterm: forall G H a,
-    AWTerm G a ->
-    ExtCtx G H ->
-    AWTerm H a
-with
-extension_weakening_awtermt : forall G H a,
-    AWTermT G a ->
-    ExtCtx G H ->
-    AWTermT H a.
+Lemma extension_weakening_awtermt : extension_weakening_awtermt_def.
 Proof.
   introv ga gh. assert (wf: ok H). apply* ok_preservation.
   gen H.
@@ -1259,31 +1251,23 @@ Proof.
   rewrite hi in wf. apply* ok_middle_inv_r.
 
   apply extension_order_typvar in gh. destruct gh as (H1 & H2 & t2 & [hi _]).
-  rewrite hi. apply* AWTerm_TypVar.
+  rewrite hi. apply* AWTermT_TypVar.
   apply* binds_middle_eq.
   rewrite hi in wf. apply* ok_middle_inv_r.
 
   assert (AWf G). apply awf_context in gh. assumption.
   assert (AWf H1). apply awf_preservation in gh. assumption.
-  apply AWTerm_Lam with (L:=L \u dom H1 \u dom G). introv notin. apply* H0.
+  apply AWTermT_Lam with (L:=L \u dom H1 \u dom G). introv notin. apply* H0.
 
   assert (AWf G). apply awf_context in gh. assumption.
   assert (AWf H1). apply awf_preservation in gh. assumption.
-  apply AWTerm_Pi with (L:=L \u dom H1 \u dom G). apply* extension_weakening_awtermt.
-  intros. apply* extension_weakening_awtermt.
+  apply AWTermT_Pi with (L:=L \u dom H1 \u dom G). apply* IHga.
+  intros. apply* H0.
 
   assert (AWf G). apply awf_context in gh. assumption.
-  assert (AWf H0). apply awf_preservation in gh. assumption.
-  apply AWTerm_Ann. apply* IHga. apply* extension_weakening_awtermt.
-
-  assert (AWf G). apply awf_context in gh. assumption.
-  assert (AWf H0). apply awf_preservation in gh. assumption.
-  apply AWTerm_Forall with (L:=L \u dom H0 \u dom G).
-  intros. apply* extension_weakening_awtermt.
-Proof.
-  introv ga gh. assert (wf: ok H). apply* ok_preservation.
-  gen H.
-  induction ga; introv gh wf; auto; try(apply split_bind_context in H; destruct H as (G1 & G2 & gi); rewrite gi in gh).
+  assert (AWf H1). apply awf_preservation in gh. assumption.
+  apply AWTermT_Forall with (L:=L \u dom H1 \u dom G).
+  intros. apply* H0.
   apply extension_order_tvar in gh. destruct gh as (H1 & H2 & [hi _]).
   rewrite hi. apply* AWTermT_TFVar.
   apply* binds_middle_eq.
@@ -1299,9 +1283,12 @@ Proof.
   rewrite hi. apply* AWTermT_Solved_EVar.
   rewrite hi in wf. apply* binds_middle_eq.
   apply* ok_middle_inv_r.
+Qed.
 
-  apply AWTermT_Expr.
-  apply* extension_weakening_awterm.
+Lemma extension_weakening_awterm: extension_weakening_awterm_def.
+Proof.
+  unfolds extension_weakening_awterm_def.
+  unfold AWTerm. intros. apply* extension_weakening_awtermt.
 Qed.
 
 Lemma extension_equality_preservation: extension_equality_preservation_def.
